@prefix dc:    <http://purl.org/dc/elements/1.1/> .
@prefix rdfs:  <http://www.w3.org/2000/01/rdf-schema#> .
@prefix dct:   <http://purl.org/dc/terms/> .
@prefix owl:   <http://www.w3.org/2002/07/owl#> .
@prefix xsd:   <http://www.w3.org/2001/XMLSchema#> .
@prefix baseInspire:  <http://portele.de/ont/inspire/baseInspire#> .
@prefix rdf:   <http://www.w3.org/1999/02/22-rdf-syntax-ns#> .
@prefix iso19150-2: <http://def.seegrid.csiro.au/isotc211/iso19150/-2/2012/basic#> .
@prefix skos:  <http://www.w3.org/2004/02/skos/core#> .
@prefix geo:   <http://www.opengis.net/ont/geosparql#> .

<http://portele.de/ont/inspire/baseInspire>
        a                owl:Ontology ;
        rdfs:comment     "Schema for basic types used by multiple themes. Removed ^^xsd:NCName from skos:notation"@en ;
        rdfs:label       "Base Types"@en ;
        dc:source        "INSPIRE application schemas, Revision 4618, derived according to ISO/DIS 19150-2 with several modification using ShapeChange."@en ;
        owl:versionInfo  "3.4" .

baseInspire:VerticalPositionValue
        a                         rdfs:Datatype ;
        iso19150-2:isEnumeration  true ;
        owl:equivalentClass				[owl:oneOf ( "underground" "suspendedOrElevated" "onGroundSurface")] ;
        skos:definition           "The relative vertical position of a spatial object."@en ;
        skos:notation             "VerticalPositionValue" ;
        skos:prefLabel            "VerticalPositionValue"@en .

baseInspire:officialJournalIdentification
        a                owl:DatatypeProperty ;
        rdfs:range       xsd:string ;
        skos:definition  "Reference to the location within the official journal within which the legislative instrument was published. This reference shall be comprised of three parts:\r\n<ul>\r\n\t<li>the title of the official journal</li>\r\n\t<li>the volume and/or series number</li>\r\n\t<li>Page number(s)</li>\r\n</ul>"@en ;
        skos:notation    "officialJournalIdentification" ;
        skos:prefLabel   "official journal identification"@en ;
        skos:scopeNote   "EXAMPLE: Official Journal of European Union (OJEU), L108, Volume 50, 1-14"@en .

baseInspire:identifier  a      owl:DatatypeProperty ;
        rdfs:range       xsd:string ;
        skos:definition  "Unique identifier used to identify a real world phenomenon within the specified identification scheme."@en ;
        skos:notation    "identifier" ;
        skos:prefLabel   "identifier"@en .

baseInspire:ThematicIdentifier
        a                owl:Class ;
        rdfs:subClassOf  iso19150-2:Datatype ;
        skos:definition  "Thematic identifier to identify the real world phenomenon of spatial object."@en ;
        skos:notation    "ThematicIdentifier" ;
        skos:prefLabel   "thematic identifier"@en ;
        skos:scopeNote   "Some real world phenomena may be assigned multiple unique identifiers. \r\nThese may have been established to meet data exchange requirements of different reporting obligations at International, European or national levels and/or internal data maintenance requirements."@en .
        
baseInspire:positionName  a    owl:DatatypeProperty ;
        rdfs:range       xsd:string ;
        skos:definition  "Position of the party in relation to a resource, such as head of department."@en ;
        skos:notation    "positionName" ;
        skos:prefLabel   "position name"@en .

baseInspire:electronicMailAddress
        a                owl:DatatypeProperty ;
        rdfs:range       xsd:string ;
        skos:definition  "An address of the organisation's or individual's electronic mailbox."@en ;
        skos:notation    "electronicMailAddress" ;
        skos:prefLabel   "electronicMailAddress"@en .

baseInspire:officialDocumentNumber
        a                owl:DatatypeProperty ;
        rdfs:range       xsd:string ;
        skos:definition  "Official document number used to uniquely identify the legislative instrument."@en ;
        skos:notation    "officialDocumentNumber" ;
        skos:prefLabel   "official document number"@en ;
        skos:scopeNote   "NOTE: An official document number may be assigned to uniquely identify the legislative instrument.\r\n\r\nEXAMPLE: CELEX Number used to uniquely identify European Union Legislation"@en .

baseInspire:contactInstructions
        a                owl:DatatypeProperty ;
        rdfs:range       xsd:string ;
        skos:definition  "Supplementary instructions on how or when to contact an individual or organisation."@en ;
        skos:notation    "contactInstructions" ;
        skos:prefLabel   "contactInstructions"@en .

baseInspire:OfficialJournalInformation
        a                owl:Class ;
        rdfs:subClassOf  iso19150-2:Datatype ;
        skos:definition  "Full citation of the location of the legislative instrument within the official journal."@en ;
        skos:notation    "OfficialJournalInformation" ;
        skos:prefLabel   "official journal information"@en .

baseInspire:linkToJournal  a   owl:DatatypeProperty ;
        rdfs:range       xsd:anyURI ;
        skos:definition  "Link to an online version of the official journal"@en ;
        skos:notation    "linkToJournal" ;
        skos:prefLabel   "link to online version"@en .

baseInspire:organisationName
        a                owl:DatatypeProperty ;
        rdfs:range       xsd:string ;
        skos:definition  "Name of the related organisation."@en ;
        skos:notation    "organisationName" ;
        skos:prefLabel   "organisation name"@en .

baseInspire:link  a            owl:DatatypeProperty ;
        rdfs:range       xsd:anyURI ;
        skos:definition  "Link to an online version of the document"@en ;
        skos:notation    "link" ;
        skos:prefLabel   "link to online version"@en .

baseInspire:telephoneVoice  a  owl:DatatypeProperty ;
        rdfs:range       xsd:string ;
        skos:definition  "Telephone number of the organisation or individual."@en ;
        skos:notation    "telephoneVoice" ;
        skos:prefLabel   "telephoneVoice"@en .

baseInspire:dateEnteredIntoForce
        a                owl:ObjectProperty ;
        rdfs:comment     "The range is a type for which no RDF representation is known: TM_Position"@en ;
        rdfs:range       owl:Thing ;
        skos:definition  "Date the legislative instrument entered into force."@en ;
        skos:notation    "dateEnteredIntoForce" ;
        skos:prefLabel   "date entered into force"@en .

baseInspire:identificationNumber
        a                owl:DatatypeProperty ;
        rdfs:range       xsd:string ;
        skos:definition  "Code used to identify the legislative instrument"@en ;
        skos:notation    "identificationNumber" ;
        skos:prefLabel   "identification number"@en ;
        skos:scopeNote   "EXAMPLE 1: 2007/2/EC is the identification number for the INSPIRE Directive\r\n\r\nEXAMPLE 2: 2008/50/EC is the identification number for the CAFE Directive\r\n\r\nEXAMPLE 3: 2000/60/EC is the identification number for the  Water Framework Directive"@en .

baseInspire:iSBN  a            owl:DatatypeProperty ;
        rdfs:range       xsd:string ;
        skos:definition  "International Standard Book Number (ISBN) is an nine-digit number that uniquely identifies the book in which the legislative instrument was published."@en ;
        skos:notation    "ISBN" ;
        skos:prefLabel   "ISBN"@en .

baseInspire:level  a           owl:ObjectProperty ;
        rdfs:comment     "The range is a type for which no RDF representation is known: LegislationLevelValue"@en ;
        rdfs:range       owl:Thing ;
        skos:definition  "The level at which the legislative instrument is adopted."@en ;
        skos:notation    "level" ;
        skos:prefLabel   "name"@en .

baseInspire:telephoneFacsimile
        a                owl:DatatypeProperty ;
        rdfs:range       xsd:string ;
        skos:definition  "Number of a facsimile machine of the organisation or individual."@en ;
        skos:notation    "telephoneFacsimile" ;
        skos:prefLabel   "telephoneFacsimile"@en .

baseInspire:specificReference
        a                owl:DatatypeProperty ;
        rdfs:range       xsd:string ;
        skos:definition  "Reference to a specific part of the document."@en ;
        skos:notation    "specificReference" ;
        skos:prefLabel   "specific reference"@en ;
        skos:scopeNote   "EXAMPLE For legal documents, this attribute can contain a reference to article(s) that specify a specific requirement or obligation."@en .

baseInspire:Contact  a         owl:Class ;
        rdfs:subClassOf  iso19150-2:Datatype ;
        skos:definition  "Communication channels by which it is possible to gain access to someone or something."@en ;
        skos:notation    "Contact" ;
        skos:prefLabel   "contact"@en .

baseInspire:LegislationCitation
        a                owl:Class ;
        rdfs:subClassOf  baseInspire:DocumentCitation , iso19150-2:Interface ;
        skos:definition  "Citation for the purposes of unambiguously referencing a legal act or a specific part of a legal act."@en ;
        skos:notation    "LegislationCitation" ;
        skos:prefLabel   "legislation citation"@en .

baseInspire:date  a            owl:ObjectProperty ;
        rdfs:comment     "The range is a type for which no RDF representation is known: CI_Date"@en ;
        rdfs:range       owl:Thing ;
        skos:definition  "Date of creation, publication or revision of the document."@en ;
        skos:notation    "date" ;
        skos:prefLabel   "date"@en .

baseInspire:individualName  a  owl:DatatypeProperty ;
        rdfs:range       xsd:string ;
        skos:definition  "Name of the related person."@en ;
        skos:notation    "individualName" ;
        skos:prefLabel   "individual name"@en .

baseInspire:DocumentCitation
        a                owl:Class ;
        rdfs:subClassOf  iso19150-2:Interface ;
        skos:definition  "Citation for the purposes of unambiguously referencing a document."@en ;
        skos:notation    "DocumentCitation" ;
        skos:prefLabel   "document citation"@en .

baseInspire:address  a         owl:ObjectProperty ;
        rdfs:comment     "The range is a type for which no RDF representation is known: AddressRepresentation"@en ;
        rdfs:range       owl:Thing ;
        skos:definition  "An address provided as free text."@en ;
        skos:notation    "address" ;
        skos:prefLabel   "address"@en .

baseInspire:role  a            owl:ObjectProperty ;
        rdfs:comment     "The range is a type for which no RDF representation is known: PartyRoleValue"@en ;
        rdfs:range       owl:Thing ;
        skos:definition  "Role(s) of the party in relation to a resource, such as owner."@en ;
        skos:notation    "role" ;
        skos:prefLabel   "role"@en .

baseInspire:iSSN  a            owl:DatatypeProperty ;
        rdfs:range       xsd:string ;
        skos:definition  "The International Standard Serial Number (ISSN) is an eight-digit number that identifies the periodical publication in which the legislative instrument was published."@en ;
        skos:notation    "ISSN" ;
        skos:prefLabel   "ISSN"@en ;
        skos:scopeNote   "NOTE: Periodical publilcations are issued in successive parts, usually having numerical or chronological designations and required that each serial publication can be uniquely identified.\r\n\r\nEXAMPLE: OJ Series in which INSPIRE Directive is published has been assigned the ISSN: 1725-2555"@en .

baseInspire:shortName  a       owl:DatatypeProperty ;
        rdfs:range       xsd:string ;
        skos:definition  "Short name or alternative title of the document."@en ;
        skos:notation    "shortName" ;
        skos:prefLabel   "short name"@en ;
        skos:scopeNote   "NOTE\tFor legal documents, this should be a short name or alternative title commonly used to identify the legislation.\r\n\r\nEXAMPLE 1: INSPIRE Directive is the short name for \"Directive 2007/2/EC of the European Parliament and of the Council of 14 March 2007 establishing an Infrastructure for Spatial Information in the European Community (INSPIRE)\"\r\n\r\nEXAMPLE 2: CAFE Directive is the short name for the Directive 2008/50/EC of the European Parliament and of the Council of 21 May 2008 on ambient air quality and cleaner air for Europe\" \r\n\r\nEXAMPLE  3: Water Framework Directive the short name for \"Directive 2000/60/EC of the European Parliament and of the Council establishing a framework for the Community action in the field of water policy\""@en .

baseInspire:journalCitation
        a                owl:ObjectProperty ;
        rdfs:range       baseInspire:OfficialJournalInformation ;
        skos:definition  "Citation of the official journal in which the legislation is published."@en ;
        skos:notation    "journalCitation" ;
        skos:prefLabel   "journal citation"@en .

baseInspire:hoursOfService  a  owl:DatatypeProperty ;
        rdfs:range       xsd:string ;
        skos:definition  "Periods of time when the organisation or individual can be contacted."@en ;
        skos:notation    "hoursOfService" ;
        skos:prefLabel   "hoursOfService"@en .

baseInspire:website  a         owl:DatatypeProperty ;
        rdfs:range       xsd:anyURI ;
        skos:definition  "Pages provided on the World Wide Web by the organisation or individual."@en ;
        skos:notation    "website" ;
        skos:prefLabel   "website"@en .

baseInspire:identifierScheme
        a                owl:DatatypeProperty ;
        rdfs:range       xsd:string ;
        skos:definition  "Identifier defining the scheme used to assign the identifier."@en ;
        skos:notation    "identifierScheme" ;
        skos:prefLabel   "identifier scheme"@en ;
        skos:scopeNote   "NOTE 1: Reporting requirements for different environmental legislation mandate that each spatial object is assigned an identifier conforming to specific lexical rules. \r\n\r\nNOTE 2: These rules are often inconsistent so a spatial object may be assigned multiple identifiers which are used for object referencing to link information to the spatial object."@en .

baseInspire:dateRepealed  a    owl:ObjectProperty ;
        rdfs:comment     "The range is a type for which no RDF representation is known: TM_Position"@en ;
        rdfs:range       owl:Thing ;
        skos:definition  "Date the legislative instrument was repealed."@en ;
        skos:notation    "dateRepealed" ;
        skos:prefLabel   "date repealed"@en .

baseInspire:RelatedParty  a    owl:Class ;
        rdfs:subClassOf  iso19150-2:Datatype ;
        skos:definition  "An organisation or a person with a role related to a resource."@en ;
        skos:notation    "RelatedParty" ;
        skos:prefLabel   "related party"@en ;
        skos:scopeNote   "NOTE 1 A party, typically an individual person, acting as a general point of contact for a resource can be specified without providing any particular role."@en .

baseInspire:contact  a         owl:ObjectProperty ;
        rdfs:range       baseInspire:Contact ;
        skos:definition  "Contact information for the related party."@en ;
        skos:notation    "contact" ;
        skos:prefLabel   "contact"@en .

baseInspire:responsibleParty  
        a                owl:ObjectProperty ;
        rdfs:range       baseInspire:RelatedParty ;
        skos:definition  "The responsible party."@en ;
        skos:notation    "responsibleParty" ;
        skos:prefLabel   "responsible Party"@en .

baseInspire:beginLifespanVersion
        a                owl:DatatypeProperty ;
        rdfs:range       xsd:dateTime ;
        skos:definition  "..."@en ;
        skos:notation    "beginLifespanVersion" ;
        skos:prefLabel   "begin of lifespan of feature version"@en .
        
baseInspire:endLifespanVersion
        a                owl:DatatypeProperty ;
        rdfs:range       xsd:dateTime ;
        skos:definition  "..."@en ;
        skos:notation    "endLifespanVersion" ;
        skos:prefLabel   "end of lifespan of feature version"@en .

baseInspire:validFrom
        a                owl:DatatypeProperty ;
        rdfs:range       xsd:dateTime ;
        skos:definition  "..."@en ;
        skos:notation    "validFrom" ;
        skos:prefLabel   "begin of real-world phenomenon"@en .
        
baseInspire:validTo
        a                owl:DatatypeProperty ;
        rdfs:range       xsd:dateTime ;
        skos:definition  "..."@en ;
        skos:notation    "validTo" ;
        skos:prefLabel   "end of real-world phenomenon"@en .

baseInspire:representativePoint
        a                owl:ObjectProperty ;
        rdfs:subPropertyOf	geo:hasGeometry ;
        rdfs:range       geo:Geometry ;
        skos:definition  "Representative location."@en ;
        skos:notation    "representativePoint" ;
        skos:prefLabel   "representative Point"@en .

baseInspire:extent
		  a          		 owl:ObjectProperty ;
        rdfs:comment     "The range is a type for which no RDF representation is known: EX_Extent"@en ;
        rdfs:range       owl:Thing ;
        skos:definition  "Information about the spatial and temporal extent."@en ;
        skos:notation    "extent" ;
        skos:prefLabel   "extent"@en .

