<?xml version="1.0"?>


<!DOCTYPE rdf:RDF [
    <!ENTITY dct "http://purl.org/dc/terms/" >
    <!ENTITY owl "http://www.w3.org/2002/07/owl#" >
    <!ENTITY dc "http://purl.org/dc/elements/1.1/" >
    <!ENTITY xsd "http://www.w3.org/2001/XMLSchema#" >
    <!ENTITY xml "http://www.w3.org/XML/1998/namespace" >
    <!ENTITY skos "http://www.w3.org/2004/02/skos/core#" >
    <!ENTITY rdfs "http://www.w3.org/2000/01/rdf-schema#" >
    <!ENTITY geo "http://www.opengis.net/ont/geosparql#" >
    <!ENTITY baseInspire "http://portele.de/ont/inspire/baseInspire#" >
    <!ENTITY rdf "http://www.w3.org/1999/02/22-rdf-syntax-ns#" >
    <!ENTITY iso19150-2 "http://def.seegrid.csiro.au/isotc211/iso19150/-2/2012/basic#" >
]>


<rdf:RDF xmlns="http://www.semanticweb.org/owl/owlapi/turtle#"
     xml:base="http://www.semanticweb.org/owl/owlapi/turtle"
     xmlns:iso19150-2="http://def.seegrid.csiro.au/isotc211/iso19150/-2/2012/basic#"
     xmlns:owl="http://www.w3.org/2002/07/owl#"
     xmlns:xsd="http://www.w3.org/2001/XMLSchema#"
     xmlns:skos="http://www.w3.org/2004/02/skos/core#"
     xmlns:rdfs="http://www.w3.org/2000/01/rdf-schema#"
     xmlns:geo="http://www.opengis.net/ont/geosparql#"
     xmlns:baseInspire="http://portele.de/ont/inspire/baseInspire#"
     xmlns:dct="http://purl.org/dc/terms/"
     xmlns:rdf="http://www.w3.org/1999/02/22-rdf-syntax-ns#"
     xmlns:xml="http://www.w3.org/XML/1998/namespace"
     xmlns:dc="http://purl.org/dc/elements/1.1/">
    <owl:Ontology rdf:about="http://portele.de/ont/inspire/baseInspire">
        <rdfs:label xml:lang="en">Base Types</rdfs:label>
        <owl:versionInfo>3.3</owl:versionInfo>
        <dc:source xml:lang="en">INSPIRE application schemas, Revision 4618, derived according to ISO/DIS 19150-2 with several modification using ShapeChange.</dc:source>
        <rdfs:comment xml:lang="en">schema for basic types used by multiple themes</rdfs:comment>
    </owl:Ontology>
    


    <!-- 
    ///////////////////////////////////////////////////////////////////////////////////////
    //
    // Annotation properties
    //
    ///////////////////////////////////////////////////////////////////////////////////////
     -->

    


    <!-- http://def.seegrid.csiro.au/isotc211/iso19150/-2/2012/basic#isEnumeration -->

    <owl:AnnotationProperty rdf:about="&iso19150-2;isEnumeration"/>
    


    <!-- http://www.w3.org/2004/02/skos/core#definition -->

    <owl:AnnotationProperty rdf:about="&skos;definition"/>
    


    <!-- http://www.w3.org/2004/02/skos/core#notation -->

    <owl:AnnotationProperty rdf:about="&skos;notation"/>
    


    <!-- http://www.w3.org/2004/02/skos/core#prefLabel -->

    <owl:AnnotationProperty rdf:about="&skos;prefLabel"/>
    


    <!-- http://www.w3.org/2004/02/skos/core#scopeNote -->

    <owl:AnnotationProperty rdf:about="&skos;scopeNote"/>
    


    <!-- 
    ///////////////////////////////////////////////////////////////////////////////////////
    //
    // Datatypes
    //
    ///////////////////////////////////////////////////////////////////////////////////////
     -->

    


    <!-- http://portele.de/ont/inspire/baseInspire#VerticalPositionValue -->

    <rdfs:Datatype rdf:about="&baseInspire;VerticalPositionValue">
        <owl:equivalentClass>
            <rdfs:Datatype>
                <owl:oneOf>
                    <rdf:Description>
                        <rdf:type rdf:resource="&rdf;List"/>
                        <rdf:first>onGroundSurface</rdf:first>
                        <rdf:rest>
                            <rdf:Description>
                                <rdf:type rdf:resource="&rdf;List"/>
                                <rdf:first>suspendedOrElevated</rdf:first>
                                <rdf:rest>
                                    <rdf:Description>
                                        <rdf:type rdf:resource="&rdf;List"/>
                                        <rdf:first>underground</rdf:first>
                                        <rdf:rest rdf:resource="&rdf;nil"/>
                                    </rdf:Description>
                                </rdf:rest>
                            </rdf:Description>
                        </rdf:rest>
                    </rdf:Description>
                </owl:oneOf>
            </rdfs:Datatype>
        </owl:equivalentClass>
        <skos:notation rdf:datatype="&xsd;NCName">VerticalPositionValue</skos:notation>
        <iso19150-2:isEnumeration rdf:datatype="&xsd;boolean">true</iso19150-2:isEnumeration>
        <skos:definition xml:lang="en">The relative vertical position of a spatial object.</skos:definition>
        <skos:prefLabel xml:lang="en">VerticalPositionValue</skos:prefLabel>
    </rdfs:Datatype>
    


    <!-- 
    ///////////////////////////////////////////////////////////////////////////////////////
    //
    // Object Properties
    //
    ///////////////////////////////////////////////////////////////////////////////////////
     -->

    


    <!-- http://portele.de/ont/inspire/baseInspire#address -->

    <owl:ObjectProperty rdf:about="&baseInspire;address">
        <skos:notation rdf:datatype="&xsd;NCName">address</skos:notation>
        <skos:definition xml:lang="en">An address provided as free text.</skos:definition>
        <rdfs:comment xml:lang="en">The range is a type for which no RDF representation is known: AddressRepresentation</rdfs:comment>
        <skos:prefLabel xml:lang="en">address</skos:prefLabel>
        <rdfs:range rdf:resource="&owl;Thing"/>
    </owl:ObjectProperty>
    


    <!-- http://portele.de/ont/inspire/baseInspire#contact -->

    <owl:ObjectProperty rdf:about="&baseInspire;contact">
        <skos:notation rdf:datatype="&xsd;NCName">contact</skos:notation>
        <skos:definition xml:lang="en">Contact information for the related party.</skos:definition>
        <skos:prefLabel xml:lang="en">contact</skos:prefLabel>
        <rdfs:range rdf:resource="&baseInspire;Contact"/>
    </owl:ObjectProperty>
    


    <!-- http://portele.de/ont/inspire/baseInspire#date -->

    <owl:ObjectProperty rdf:about="&baseInspire;date">
        <skos:notation rdf:datatype="&xsd;NCName">date</skos:notation>
        <skos:definition xml:lang="en">Date of creation, publication or revision of the document.</skos:definition>
        <rdfs:comment xml:lang="en">The range is a type for which no RDF representation is known: CI_Date</rdfs:comment>
        <skos:prefLabel xml:lang="en">date</skos:prefLabel>
        <rdfs:range rdf:resource="&owl;Thing"/>
    </owl:ObjectProperty>
    


    <!-- http://portele.de/ont/inspire/baseInspire#dateEnteredIntoForce -->

    <owl:ObjectProperty rdf:about="&baseInspire;dateEnteredIntoForce">
        <skos:notation rdf:datatype="&xsd;NCName">dateEnteredIntoForce</skos:notation>
        <skos:definition xml:lang="en">Date the legislative instrument entered into force.</skos:definition>
        <rdfs:comment xml:lang="en">The range is a type for which no RDF representation is known: TM_Position</rdfs:comment>
        <skos:prefLabel xml:lang="en">date entered into force</skos:prefLabel>
        <rdfs:range rdf:resource="&owl;Thing"/>
    </owl:ObjectProperty>
    


    <!-- http://portele.de/ont/inspire/baseInspire#dateRepealed -->

    <owl:ObjectProperty rdf:about="&baseInspire;dateRepealed">
        <skos:notation rdf:datatype="&xsd;NCName">dateRepealed</skos:notation>
        <skos:definition xml:lang="en">Date the legislative instrument was repealed.</skos:definition>
        <rdfs:comment xml:lang="en">The range is a type for which no RDF representation is known: TM_Position</rdfs:comment>
        <skos:prefLabel xml:lang="en">date repealed</skos:prefLabel>
        <rdfs:range rdf:resource="&owl;Thing"/>
    </owl:ObjectProperty>
    


    <!-- http://portele.de/ont/inspire/baseInspire#extent -->

    <owl:ObjectProperty rdf:about="&baseInspire;extent">
        <skos:notation rdf:datatype="&xsd;NCName">extent</skos:notation>
        <skos:definition xml:lang="en">Information about the spatial and temporal extent.</skos:definition>
        <rdfs:comment xml:lang="en">The range is a type for which no RDF representation is known: EX_Extent</rdfs:comment>
        <skos:prefLabel xml:lang="en">extent</skos:prefLabel>
        <rdfs:range rdf:resource="&owl;Thing"/>
    </owl:ObjectProperty>
    


    <!-- http://portele.de/ont/inspire/baseInspire#journalCitation -->

    <owl:ObjectProperty rdf:about="&baseInspire;journalCitation">
        <skos:notation rdf:datatype="&xsd;NCName">journalCitation</skos:notation>
        <skos:definition xml:lang="en">Citation of the official journal in which the legislation is published.</skos:definition>
        <skos:prefLabel xml:lang="en">journal citation</skos:prefLabel>
        <rdfs:range rdf:resource="&baseInspire;OfficialJournalInformation"/>
    </owl:ObjectProperty>
    


    <!-- http://portele.de/ont/inspire/baseInspire#level -->

    <owl:ObjectProperty rdf:about="&baseInspire;level">
        <skos:notation rdf:datatype="&xsd;NCName">level</skos:notation>
        <skos:definition xml:lang="en">The level at which the legislative instrument is adopted.</skos:definition>
        <rdfs:comment xml:lang="en">The range is a type for which no RDF representation is known: LegislationLevelValue</rdfs:comment>
        <skos:prefLabel xml:lang="en">name</skos:prefLabel>
        <rdfs:range rdf:resource="&owl;Thing"/>
    </owl:ObjectProperty>
    


    <!-- http://portele.de/ont/inspire/baseInspire#representativePoint -->

    <owl:ObjectProperty rdf:about="&baseInspire;representativePoint">
        <skos:notation rdf:datatype="&xsd;NCName">representativePoint</skos:notation>
        <skos:definition xml:lang="en">Representative location.</skos:definition>
        <skos:prefLabel xml:lang="en">representative Point</skos:prefLabel>
        <rdfs:range rdf:resource="&geo;Geometry"/>
        <rdfs:subPropertyOf rdf:resource="&geo;hasGeometry"/>
    </owl:ObjectProperty>
    


    <!-- http://portele.de/ont/inspire/baseInspire#responsibleParty -->

    <owl:ObjectProperty rdf:about="&baseInspire;responsibleParty">
        <skos:notation rdf:datatype="&xsd;NCName">responsibleParty</skos:notation>
        <skos:definition xml:lang="en">The responsible party.</skos:definition>
        <skos:prefLabel xml:lang="en">responsible Party</skos:prefLabel>
        <rdfs:range rdf:resource="&baseInspire;RelatedParty"/>
    </owl:ObjectProperty>
    


    <!-- http://portele.de/ont/inspire/baseInspire#role -->

    <owl:ObjectProperty rdf:about="&baseInspire;role">
        <skos:notation rdf:datatype="&xsd;NCName">role</skos:notation>
        <skos:definition xml:lang="en">Role(s) of the party in relation to a resource, such as owner.</skos:definition>
        <rdfs:comment xml:lang="en">The range is a type for which no RDF representation is known: PartyRoleValue</rdfs:comment>
        <skos:prefLabel xml:lang="en">role</skos:prefLabel>
        <rdfs:range rdf:resource="&owl;Thing"/>
    </owl:ObjectProperty>
    


    <!-- http://www.opengis.net/ont/geosparql#hasGeometry -->

    <owl:ObjectProperty rdf:about="&geo;hasGeometry"/>
    


    <!-- 
    ///////////////////////////////////////////////////////////////////////////////////////
    //
    // Data properties
    //
    ///////////////////////////////////////////////////////////////////////////////////////
     -->

    


    <!-- http://portele.de/ont/inspire/baseInspire#beginLifespanVersion -->

    <owl:DatatypeProperty rdf:about="&baseInspire;beginLifespanVersion">
        <skos:notation rdf:datatype="&xsd;NCName">beginLifespanVersion</skos:notation>
        <skos:definition xml:lang="en">...</skos:definition>
        <skos:prefLabel xml:lang="en">begin of lifespan of feature version</skos:prefLabel>
        <rdfs:range rdf:resource="&xsd;dateTime"/>
    </owl:DatatypeProperty>
    


    <!-- http://portele.de/ont/inspire/baseInspire#contactInstructions -->

    <owl:DatatypeProperty rdf:about="&baseInspire;contactInstructions">
        <skos:notation rdf:datatype="&xsd;NCName">contactInstructions</skos:notation>
        <skos:definition xml:lang="en">Supplementary instructions on how or when to contact an individual or organisation.</skos:definition>
        <skos:prefLabel xml:lang="en">contactInstructions</skos:prefLabel>
        <rdfs:range rdf:resource="&xsd;string"/>
    </owl:DatatypeProperty>
    


    <!-- http://portele.de/ont/inspire/baseInspire#electronicMailAddress -->

    <owl:DatatypeProperty rdf:about="&baseInspire;electronicMailAddress">
        <skos:notation rdf:datatype="&xsd;NCName">electronicMailAddress</skos:notation>
        <skos:definition xml:lang="en">An address of the organisation&apos;s or individual&apos;s electronic mailbox.</skos:definition>
        <skos:prefLabel xml:lang="en">electronicMailAddress</skos:prefLabel>
        <rdfs:range rdf:resource="&xsd;string"/>
    </owl:DatatypeProperty>
    


    <!-- http://portele.de/ont/inspire/baseInspire#endLifespanVersion -->

    <owl:DatatypeProperty rdf:about="&baseInspire;endLifespanVersion">
        <skos:notation rdf:datatype="&xsd;NCName">endLifespanVersion</skos:notation>
        <skos:definition xml:lang="en">...</skos:definition>
        <skos:prefLabel xml:lang="en">end of lifespan of feature version</skos:prefLabel>
        <rdfs:range rdf:resource="&xsd;dateTime"/>
    </owl:DatatypeProperty>
    


    <!-- http://portele.de/ont/inspire/baseInspire#hoursOfService -->

    <owl:DatatypeProperty rdf:about="&baseInspire;hoursOfService">
        <skos:notation rdf:datatype="&xsd;NCName">hoursOfService</skos:notation>
        <skos:definition xml:lang="en">Periods of time when the organisation or individual can be contacted.</skos:definition>
        <skos:prefLabel xml:lang="en">hoursOfService</skos:prefLabel>
        <rdfs:range rdf:resource="&xsd;string"/>
    </owl:DatatypeProperty>
    


    <!-- http://portele.de/ont/inspire/baseInspire#iSBN -->

    <owl:DatatypeProperty rdf:about="&baseInspire;iSBN">
        <skos:notation rdf:datatype="&xsd;NCName">ISBN</skos:notation>
        <skos:prefLabel xml:lang="en">ISBN</skos:prefLabel>
        <skos:definition xml:lang="en">International Standard Book Number (ISBN) is an nine-digit number that uniquely identifies the book in which the legislative instrument was published.</skos:definition>
        <rdfs:range rdf:resource="&xsd;string"/>
    </owl:DatatypeProperty>
    


    <!-- http://portele.de/ont/inspire/baseInspire#iSSN -->

    <owl:DatatypeProperty rdf:about="&baseInspire;iSSN">
        <skos:notation rdf:datatype="&xsd;NCName">ISSN</skos:notation>
        <skos:prefLabel xml:lang="en">ISSN</skos:prefLabel>
        <skos:scopeNote xml:lang="en">NOTE: Periodical publilcations are issued in successive parts, usually having numerical or chronological designations and required that each serial publication can be uniquely identified.rnrnEXAMPLE: OJ Series in which INSPIRE Directive is published has been assigned the ISSN: 1725-2555</skos:scopeNote>
        <skos:definition xml:lang="en">The International Standard Serial Number (ISSN) is an eight-digit number that identifies the periodical publication in which the legislative instrument was published.</skos:definition>
        <rdfs:range rdf:resource="&xsd;string"/>
    </owl:DatatypeProperty>
    


    <!-- http://portele.de/ont/inspire/baseInspire#identificationNumber -->

    <owl:DatatypeProperty rdf:about="&baseInspire;identificationNumber">
        <skos:notation rdf:datatype="&xsd;NCName">identificationNumber</skos:notation>
        <skos:definition xml:lang="en">Code used to identify the legislative instrument</skos:definition>
        <skos:scopeNote xml:lang="en">EXAMPLE 1: 2007/2/EC is the identification number for the INSPIRE DirectivernrnEXAMPLE 2: 2008/50/EC is the identification number for the CAFE DirectivernrnEXAMPLE 3: 2000/60/EC is the identification number for the  Water Framework Directive</skos:scopeNote>
        <skos:prefLabel xml:lang="en">identification number</skos:prefLabel>
        <rdfs:range rdf:resource="&xsd;string"/>
    </owl:DatatypeProperty>
    


    <!-- http://portele.de/ont/inspire/baseInspire#identifier -->

    <owl:DatatypeProperty rdf:about="&baseInspire;identifier">
        <skos:notation rdf:datatype="&xsd;NCName">identifier</skos:notation>
        <skos:definition xml:lang="en">Unique identifier used to identify a real world phenomenon within the specified identification scheme.</skos:definition>
        <skos:prefLabel xml:lang="en">identifier</skos:prefLabel>
        <rdfs:range rdf:resource="&xsd;string"/>
    </owl:DatatypeProperty>
    


    <!-- http://portele.de/ont/inspire/baseInspire#identifierScheme -->

    <owl:DatatypeProperty rdf:about="&baseInspire;identifierScheme">
        <skos:notation rdf:datatype="&xsd;NCName">identifierScheme</skos:notation>
        <skos:definition xml:lang="en">Identifier defining the scheme used to assign the identifier.</skos:definition>
        <skos:scopeNote xml:lang="en">NOTE 1: Reporting requirements for different environmental legislation mandate that each spatial object is assigned an identifier conforming to specific lexical rules. rnrnNOTE 2: These rules are often inconsistent so a spatial object may be assigned multiple identifiers which are used for object referencing to link information to the spatial object.</skos:scopeNote>
        <skos:prefLabel xml:lang="en">identifier scheme</skos:prefLabel>
        <rdfs:range rdf:resource="&xsd;string"/>
    </owl:DatatypeProperty>
    


    <!-- http://portele.de/ont/inspire/baseInspire#individualName -->

    <owl:DatatypeProperty rdf:about="&baseInspire;individualName">
        <skos:notation rdf:datatype="&xsd;NCName">individualName</skos:notation>
        <skos:definition xml:lang="en">Name of the related person.</skos:definition>
        <skos:prefLabel xml:lang="en">individual name</skos:prefLabel>
        <rdfs:range rdf:resource="&xsd;string"/>
    </owl:DatatypeProperty>
    


    <!-- http://portele.de/ont/inspire/baseInspire#link -->

    <owl:DatatypeProperty rdf:about="&baseInspire;link">
        <skos:notation rdf:datatype="&xsd;NCName">link</skos:notation>
        <skos:definition xml:lang="en">Link to an online version of the document</skos:definition>
        <skos:prefLabel xml:lang="en">link to online version</skos:prefLabel>
        <rdfs:range rdf:resource="&xsd;anyURI"/>
    </owl:DatatypeProperty>
    


    <!-- http://portele.de/ont/inspire/baseInspire#linkToJournal -->

    <owl:DatatypeProperty rdf:about="&baseInspire;linkToJournal">
        <skos:notation rdf:datatype="&xsd;NCName">linkToJournal</skos:notation>
        <skos:definition xml:lang="en">Link to an online version of the official journal</skos:definition>
        <skos:prefLabel xml:lang="en">link to online version</skos:prefLabel>
        <rdfs:range rdf:resource="&xsd;anyURI"/>
    </owl:DatatypeProperty>
    


    <!-- http://portele.de/ont/inspire/baseInspire#officialDocumentNumber -->

    <owl:DatatypeProperty rdf:about="&baseInspire;officialDocumentNumber">
        <skos:notation rdf:datatype="&xsd;NCName">officialDocumentNumber</skos:notation>
        <skos:scopeNote xml:lang="en">NOTE: An official document number may be assigned to uniquely identify the legislative instrument.rnrnEXAMPLE: CELEX Number used to uniquely identify European Union Legislation</skos:scopeNote>
        <skos:definition xml:lang="en">Official document number used to uniquely identify the legislative instrument.</skos:definition>
        <skos:prefLabel xml:lang="en">official document number</skos:prefLabel>
        <rdfs:range rdf:resource="&xsd;string"/>
    </owl:DatatypeProperty>
    


    <!-- http://portele.de/ont/inspire/baseInspire#officialJournalIdentification -->

    <owl:DatatypeProperty rdf:about="&baseInspire;officialJournalIdentification">
        <skos:notation rdf:datatype="&xsd;NCName">officialJournalIdentification</skos:notation>
        <skos:scopeNote xml:lang="en">EXAMPLE: Official Journal of European Union (OJEU), L108, Volume 50, 1-14</skos:scopeNote>
        <skos:definition xml:lang="en">Reference to the location within the official journal within which the legislative instrument was published. This reference shall be comprised of three parts:rn&lt;ul&gt;rnt&lt;li&gt;the title of the official journal&lt;/li&gt;rnt&lt;li&gt;the volume and/or series number&lt;/li&gt;rnt&lt;li&gt;Page number(s)&lt;/li&gt;rn&lt;/ul&gt;</skos:definition>
        <skos:prefLabel xml:lang="en">official journal identification</skos:prefLabel>
        <rdfs:range rdf:resource="&xsd;string"/>
    </owl:DatatypeProperty>
    


    <!-- http://portele.de/ont/inspire/baseInspire#organisationName -->

    <owl:DatatypeProperty rdf:about="&baseInspire;organisationName">
        <skos:notation rdf:datatype="&xsd;NCName">organisationName</skos:notation>
        <skos:definition xml:lang="en">Name of the related organisation.</skos:definition>
        <skos:prefLabel xml:lang="en">organisation name</skos:prefLabel>
        <rdfs:range rdf:resource="&xsd;string"/>
    </owl:DatatypeProperty>
    


    <!-- http://portele.de/ont/inspire/baseInspire#positionName -->

    <owl:DatatypeProperty rdf:about="&baseInspire;positionName">
        <skos:notation rdf:datatype="&xsd;NCName">positionName</skos:notation>
        <skos:definition xml:lang="en">Position of the party in relation to a resource, such as head of department.</skos:definition>
        <skos:prefLabel xml:lang="en">position name</skos:prefLabel>
        <rdfs:range rdf:resource="&xsd;string"/>
    </owl:DatatypeProperty>
    


    <!-- http://portele.de/ont/inspire/baseInspire#shortName -->

    <owl:DatatypeProperty rdf:about="&baseInspire;shortName">
        <skos:notation rdf:datatype="&xsd;NCName">shortName</skos:notation>
        <skos:scopeNote xml:lang="en">NOTEtFor legal documents, this should be a short name or alternative title commonly used to identify the legislation.rnrnEXAMPLE 1: INSPIRE Directive is the short name for &quot;Directive 2007/2/EC of the European Parliament and of the Council of 14 March 2007 establishing an Infrastructure for Spatial Information in the European Community (INSPIRE)&quot;rnrnEXAMPLE 2: CAFE Directive is the short name for the Directive 2008/50/EC of the European Parliament and of the Council of 21 May 2008 on ambient air quality and cleaner air for Europe&quot; rnrnEXAMPLE  3: Water Framework Directive the short name for &quot;Directive 2000/60/EC of the European Parliament and of the Council establishing a framework for the Community action in the field of water policy&quot;</skos:scopeNote>
        <skos:definition xml:lang="en">Short name or alternative title of the document.</skos:definition>
        <skos:prefLabel xml:lang="en">short name</skos:prefLabel>
        <rdfs:range rdf:resource="&xsd;string"/>
    </owl:DatatypeProperty>
    


    <!-- http://portele.de/ont/inspire/baseInspire#specificReference -->

    <owl:DatatypeProperty rdf:about="&baseInspire;specificReference">
        <skos:notation rdf:datatype="&xsd;NCName">specificReference</skos:notation>
        <skos:scopeNote xml:lang="en">EXAMPLE For legal documents, this attribute can contain a reference to article(s) that specify a specific requirement or obligation.</skos:scopeNote>
        <skos:definition xml:lang="en">Reference to a specific part of the document.</skos:definition>
        <skos:prefLabel xml:lang="en">specific reference</skos:prefLabel>
        <rdfs:range rdf:resource="&xsd;string"/>
    </owl:DatatypeProperty>
    


    <!-- http://portele.de/ont/inspire/baseInspire#telephoneFacsimile -->

    <owl:DatatypeProperty rdf:about="&baseInspire;telephoneFacsimile">
        <skos:notation rdf:datatype="&xsd;NCName">telephoneFacsimile</skos:notation>
        <skos:definition xml:lang="en">Number of a facsimile machine of the organisation or individual.</skos:definition>
        <skos:prefLabel xml:lang="en">telephoneFacsimile</skos:prefLabel>
        <rdfs:range rdf:resource="&xsd;string"/>
    </owl:DatatypeProperty>
    


    <!-- http://portele.de/ont/inspire/baseInspire#telephoneVoice -->

    <owl:DatatypeProperty rdf:about="&baseInspire;telephoneVoice">
        <skos:notation rdf:datatype="&xsd;NCName">telephoneVoice</skos:notation>
        <skos:definition xml:lang="en">Telephone number of the organisation or individual.</skos:definition>
        <skos:prefLabel xml:lang="en">telephoneVoice</skos:prefLabel>
        <rdfs:range rdf:resource="&xsd;string"/>
    </owl:DatatypeProperty>
    


    <!-- http://portele.de/ont/inspire/baseInspire#validFrom -->

    <owl:DatatypeProperty rdf:about="&baseInspire;validFrom">
        <skos:notation rdf:datatype="&xsd;NCName">validFrom</skos:notation>
        <skos:definition xml:lang="en">...</skos:definition>
        <skos:prefLabel xml:lang="en">begin of real-world phenomenon</skos:prefLabel>
        <rdfs:range rdf:resource="&xsd;dateTime"/>
    </owl:DatatypeProperty>
    


    <!-- http://portele.de/ont/inspire/baseInspire#validTo -->

    <owl:DatatypeProperty rdf:about="&baseInspire;validTo">
        <skos:notation rdf:datatype="&xsd;NCName">validTo</skos:notation>
        <skos:definition xml:lang="en">...</skos:definition>
        <skos:prefLabel xml:lang="en">end of real-world phenomenon</skos:prefLabel>
        <rdfs:range rdf:resource="&xsd;dateTime"/>
    </owl:DatatypeProperty>
    


    <!-- http://portele.de/ont/inspire/baseInspire#website -->

    <owl:DatatypeProperty rdf:about="&baseInspire;website">
        <skos:notation rdf:datatype="&xsd;NCName">website</skos:notation>
        <skos:definition xml:lang="en">Pages provided on the World Wide Web by the organisation or individual.</skos:definition>
        <skos:prefLabel xml:lang="en">website</skos:prefLabel>
        <rdfs:range rdf:resource="&xsd;anyURI"/>
    </owl:DatatypeProperty>
    


    <!-- 
    ///////////////////////////////////////////////////////////////////////////////////////
    //
    // Classes
    //
    ///////////////////////////////////////////////////////////////////////////////////////
     -->

    


    <!-- http://def.seegrid.csiro.au/isotc211/iso19150/-2/2012/basic#Datatype -->

    <owl:Class rdf:about="&iso19150-2;Datatype"/>
    


    <!-- http://def.seegrid.csiro.au/isotc211/iso19150/-2/2012/basic#Interface -->

    <owl:Class rdf:about="&iso19150-2;Interface"/>
    


    <!-- http://portele.de/ont/inspire/baseInspire#Contact -->

    <owl:Class rdf:about="&baseInspire;Contact">
        <rdfs:subClassOf rdf:resource="&iso19150-2;Datatype"/>
        <skos:notation rdf:datatype="&xsd;NCName">Contact</skos:notation>
        <skos:definition xml:lang="en">Communication channels by which it is possible to gain access to someone or something.</skos:definition>
        <skos:prefLabel xml:lang="en">contact</skos:prefLabel>
    </owl:Class>
    


    <!-- http://portele.de/ont/inspire/baseInspire#DocumentCitation -->

    <owl:Class rdf:about="&baseInspire;DocumentCitation">
        <rdfs:subClassOf rdf:resource="&iso19150-2;Interface"/>
        <skos:notation rdf:datatype="&xsd;NCName">DocumentCitation</skos:notation>
        <skos:definition xml:lang="en">Citation for the purposes of unambiguously referencing a document.</skos:definition>
        <skos:prefLabel xml:lang="en">document citation</skos:prefLabel>
    </owl:Class>
    


    <!-- http://portele.de/ont/inspire/baseInspire#LegislationCitation -->

    <owl:Class rdf:about="&baseInspire;LegislationCitation">
        <rdfs:subClassOf rdf:resource="&iso19150-2;Interface"/>
        <rdfs:subClassOf rdf:resource="&baseInspire;DocumentCitation"/>
        <skos:notation rdf:datatype="&xsd;NCName">LegislationCitation</skos:notation>
        <skos:definition xml:lang="en">Citation for the purposes of unambiguously referencing a legal act or a specific part of a legal act.</skos:definition>
        <skos:prefLabel xml:lang="en">legislation citation</skos:prefLabel>
    </owl:Class>
    


    <!-- http://portele.de/ont/inspire/baseInspire#OfficialJournalInformation -->

    <owl:Class rdf:about="&baseInspire;OfficialJournalInformation">
        <rdfs:subClassOf rdf:resource="&iso19150-2;Datatype"/>
        <skos:notation rdf:datatype="&xsd;NCName">OfficialJournalInformation</skos:notation>
        <skos:definition xml:lang="en">Full citation of the location of the legislative instrument within the official journal.</skos:definition>
        <skos:prefLabel xml:lang="en">official journal information</skos:prefLabel>
    </owl:Class>
    


    <!-- http://portele.de/ont/inspire/baseInspire#RelatedParty -->

    <owl:Class rdf:about="&baseInspire;RelatedParty">
        <rdfs:subClassOf rdf:resource="&iso19150-2;Datatype"/>
        <skos:notation rdf:datatype="&xsd;NCName">RelatedParty</skos:notation>
        <skos:definition xml:lang="en">An organisation or a person with a role related to a resource.</skos:definition>
        <skos:scopeNote xml:lang="en">NOTE 1 A party, typically an individual person, acting as a general point of contact for a resource can be specified without providing any particular role.</skos:scopeNote>
        <skos:prefLabel xml:lang="en">related party</skos:prefLabel>
    </owl:Class>
    


    <!-- http://portele.de/ont/inspire/baseInspire#ThematicIdentifier -->

    <owl:Class rdf:about="&baseInspire;ThematicIdentifier">
        <rdfs:subClassOf rdf:resource="&iso19150-2;Datatype"/>
        <skos:notation rdf:datatype="&xsd;NCName">ThematicIdentifier</skos:notation>
        <skos:scopeNote xml:lang="en">Some real world phenomena may be assigned multiple unique identifiers. rnThese may have been established to meet data exchange requirements of different reporting obligations at International, European or national levels and/or internal data maintenance requirements.</skos:scopeNote>
        <skos:definition xml:lang="en">Thematic identifier to identify the real world phenomenon of spatial object.</skos:definition>
        <skos:prefLabel xml:lang="en">thematic identifier</skos:prefLabel>
    </owl:Class>
    


    <!-- http://www.opengis.net/ont/geosparql#Geometry -->

    <owl:Class rdf:about="&geo;Geometry"/>
</rdf:RDF>



<!-- Generated by the OWL API (version 3.4.2) http://owlapi.sourceforge.net -->

