# baseURI: http://def.seegrid.csiro.au/isotc211/iso19150/-2/2012/basic
# imports: http://purl.org/dc/elements/1.1/

@prefix dc: <http://purl.org/dc/elements/1.1/> .
@prefix dct: <http://purl.org/dc/terms/> .
@prefix h2o: <http://def.seegrid.csiro.au/isotc211/iso19150/-2/2012/basic#> .
@prefix owl: <http://www.w3.org/2002/07/owl#> .
@prefix prov-dc: <http://www.w3.org/ns/prov-dc#> .
@prefix rdf: <http://www.w3.org/1999/02/22-rdf-syntax-ns#> .
@prefix rdfs: <http://www.w3.org/2000/01/rdf-schema#> .
@prefix skos: <http://www.w3.org/2004/02/skos/core#> .
@prefix vann: <http://purl.org/vocab/vann/> .
@prefix voaf: <http://purl.org/vocommons/voaf#> .
@prefix xsd: <http://www.w3.org/2001/XMLSchema#> .

<http://def.seegrid.csiro.au/isotc211/iso19150/-2/2012/basic>
  rdf:type voaf:Vocabulary ;
  rdf:type owl:Ontology ;
  dc:contributor "ISO/TC 211 Project Team 19150-2"^^xsd:string ;
  dc:creator """Simon J D COX
CSIRO Australia"""^^xsd:string ;
  dc:description "This ontology establishes classes corresponding to stereotypes used in ISO-conformant models, as used in the rules for conversion of the ISO TC 211 Harmonized Model from the UML to OWL representations"^^xsd:string ;
  dc:rights "Copyright Â© 2012-2013 CSIRO"^^xsd:string ;
  dc:title "Ontology elements required for conversion of ISO/TC 211 Harmonized Model to OWL"^^xsd:string ;
  dct:created "2012-06-04T00:00:00"^^xsd:dateTime ;
  dct:hasPart h2o:ISOClassName ;
  dct:hasPart h2o:TaggedValue ;
  dct:hasPart h2o:constraint ;
  dct:hasPart h2o:isAbstract ;
  dct:hasPart h2o:tag ;
  dct:hasPart h2o:ttag ;
  dct:hasPart h2o:tvalue ;
  dct:license <http://creativecommons.org/licenses/by/3.0/> ;
  dct:modified "2014-01-07T00:00:00"^^xsd:dateTime ;
  vann:preferredNamespacePrefix "h2o"^^xsd:string ;
  vann:preferredNamespaceUri h2o: ;
  rdfs:comment """This ontology establishes classes corresponding to stereotypes used in ISO-conformant models, as used in the rules for conversion of the ISO TC 211 Harmonized Model from the UML to OWL representations. 

This vocabulary is provisional, pending finalization of ISO 19150-2.

The URI stem http://def.seegrid.csiro.au/isotc211/ is temporary. The vocabulary is expected to be ultimately published in the domain http://def.isotc211.org/ ."""^^xsd:string ;
  owl:imports dc: ;
  owl:priorVersion <https://www.seegrid.csiro.au/subversion/xmml/ontologies/tags/201305/ISOTC211/HM/hm2owl.rdf> ;
  owl:versionIRI <https://www.seegrid.csiro.au/subversion/xmml/ontologies/tags/201311/ISOTC211/HM/iso19150/-2/2012/basic.rdf> ;
.
h2o:ISOClassName
  rdf:type rdfs:Datatype ;
  rdfs:comment "A datatype for skos:notation annotations, used to indicate the original UML class name"^^xsd:string ;
  rdfs:isDefinedBy <http://def.seegrid.csiro.au/isotc211/iso19150/-2/2012/basic> ;
  rdfs:label "ISO Class name"^^xsd:string ;
  owl:equivalentClass [
      rdf:type rdfs:Datatype ;
      owl:onDataType xsd:string ;
      owl:withRestrictions (
          [
            xsd:pattern "^[A-Z]\\w*" ;
          ]
        ) ;
    ] ;
.
h2o:TaggedValue
  rdf:type owl:Class ;
  rdfs:comment "Class for UML tagged values"^^xsd:string ;
  rdfs:isDefinedBy <http://def.seegrid.csiro.au/isotc211/iso19150/-2/2012/basic> ;
  rdfs:label "UML tagged value structure"^^xsd:string ;
  rdfs:subClassOf owl:Thing ;
  rdfs:subClassOf [
      rdf:type owl:Restriction ;
      owl:cardinality "1"^^xsd:nonNegativeInteger ;
      owl:onProperty h2o:ttag ;
    ] ;
  rdfs:subClassOf [
      rdf:type owl:Restriction ;
      owl:cardinality "1"^^xsd:nonNegativeInteger ;
      owl:onProperty h2o:tvalue ;
    ] ;
.
h2o:constraint
  rdf:type owl:AnnotationProperty ;
  rdfs:isDefinedBy <http://def.seegrid.csiro.au/isotc211/iso19150/-2/2012/basic> ;
  rdfs:label "UML constraint"^^xsd:string ;
  rdfs:range xsd:string ;
.
h2o:isAbstract
  rdf:type owl:AnnotationProperty ;
  rdfs:comment "This property indicates whether the class was flagged 'abstract' in the UML model. Abstract classes cannot be instantiated directly. Concrete subclasses may be instantiated."^^xsd:string ;
  rdfs:isDefinedBy <http://def.seegrid.csiro.au/isotc211/iso19150/-2/2012/basic> ;
  rdfs:label "UML abstract class"^^xsd:string ;
  rdfs:range xsd:boolean ;
.
h2o:tag
  rdf:type owl:AnnotationProperty ;
  rdfs:comment "OWL property that links to a tagged value"^^xsd:string ;
  rdfs:isDefinedBy <http://def.seegrid.csiro.au/isotc211/iso19150/-2/2012/basic> ;
  rdfs:label "UML tagged value"^^xsd:string ;
  rdfs:range h2o:TaggedValue ;
.
h2o:ttag
  rdf:type owl:DatatypeProperty ;
  rdfs:domain h2o:TaggedValue ;
  rdfs:isDefinedBy <http://def.seegrid.csiro.au/isotc211/iso19150/-2/2012/basic> ;
  rdfs:label "UML tagged value tag"^^xsd:string ;
  rdfs:range xsd:string ;
.
h2o:tvalue
  rdf:type owl:DatatypeProperty ;
  rdfs:domain h2o:TaggedValue ;
  rdfs:isDefinedBy <http://def.seegrid.csiro.au/isotc211/iso19150/-2/2012/basic> ;
  rdfs:label "UML tagged value value"^^xsd:string ;
  rdfs:range xsd:string ;
.
h2o:valueAssignment
  rdf:type owl:ObjectProperty ;
  rdfs:comment "property that can be attached to any statement to support a link to the evidence for the value"^^xsd:string ;
  rdfs:domain rdf:Statement ;
  rdfs:label "value assignment method"^^xsd:string ;
.
